src/runtime/uv/system.h
@@ -41,5 +41,6 @@ extern "C" LEAN_EXPORT lean_obj_res lean_uv_get_total_memory();
 extern "C" LEAN_EXPORT lean_obj_res lean_uv_get_constrained_memory();
 extern "C" LEAN_EXPORT lean_obj_res lean_uv_get_available_memory();
 extern "C" LEAN_EXPORT lean_obj_res lean_uv_realpath(b_obj_arg path);
+extern "C" LEAN_EXPORT lean_obj_res lean_uv_is_symlink(b_obj_arg path);
 
 }
